fix programs.v

refinedVST/typing/programs.v
@@ -238,8 +238,8 @@ Section judgements.
               rho = construct_rho (filter_genv ge) ve te ->
               Clight.eval_expr ge ve te m e v (*/\ typeof e = t /\ tc_val t v*)⌝.*)
 
-  Definition typed_val_expr f (e : expr) (T : Ctypes.type → val → type → assert) : assert :=
-    (∀ Φ, (∀ cty v (ty : type), ⎡(valinject cty v) ◁ᵥ|cty| ty⎤ -∗ T cty v ty -∗ Φ v) -∗ wp_expr ge ⊤ f e Φ).
+  Definition typed_val_expr f (e : expr) (T : val → type → assert) : assert :=
+    (∀ Φ, (∀ v (ty : type), ⎡v ◁ᵥₐₗ|typeof e| ty⎤ -∗ T v ty -∗ Φ v) -∗ wp_expr ge ⊤ f e Φ).
   Global Arguments typed_val_expr _ _%_I.
 
   (* FIXME sounds like typed_addr_of, although typed_addr_of is for typing `&e`; are they the same?  *)
@@ -253,23 +253,23 @@ Section judgements.
   Class TypedLvalue f β (e : expr) : Type :=
     typed_lvalue_proof T : iProp_to_Prop (typed_lvalue f β e T).
 
-  Definition typed_value (v : val) (T : type → assert) : assert :=
-    (∃ cty (ty: type), ⎡(valinject cty v) ◁ᵥ|cty| ty⎤ ∗ T ty).
-  Class TypedValue (v : val) : Type :=
-    typed_value_proof T : iProp_to_Prop (typed_value v T).
+  Definition typed_value (cty : Ctypes.type) (v : val) (T : type → assert) : assert :=
+    (∃ (ty: type), ⎡v ◁ᵥₐₗ|cty| ty⎤ ∗ T ty).
+  Class TypedValue (cty : Ctypes.type) (v : val) : Type :=
+    typed_value_proof T : iProp_to_Prop (typed_value cty v T).
 
-  Definition typed_val_binop op t1 v1 t2 v2 (T : val → type → assert) : assert :=
-    (∀ Φ, (∀ cty v (ty : type), ⎡(valinject cty v) ◁ᵥ|cty| ty⎤  -∗ T v ty -∗ Φ v) -∗ wp_binop ge ⊤ op t1 v1 t2 v2 Φ).
-  Global Arguments typed_val_binop _ _ _ _ _ _%_I.
+  Definition typed_val_binop op t1 v1 t2 v2 cty (T : val → type → assert) : assert :=
+    (∀ Φ, (∀ v (ty : type), ⎡v ◁ᵥₐₗ|cty| ty⎤  -∗ T v ty -∗ Φ v) -∗ wp_binop ge ⊤ op t1 v1 t2 v2 Φ).
+  Global Arguments typed_val_binop _ _ _ _ _ _ _%_I.
 
-  Definition typed_bin_op (v1 : val) (P1 : assert) (v2 : val) (P2 : assert) (o : Cop.binary_operation) (t1 t2 : Ctypes.type) (T : val → type → assert) : assert :=
-    (P1 -∗ P2 -∗ typed_val_binop o t1 v1 t2 v2 T)%I.
+  Definition typed_bin_op (v1 : val) (P1 : assert) (v2 : val) (P2 : assert) (o : Cop.binary_operation) (t1 t2 t: Ctypes.type) (T : val → type → assert) : assert :=
+    (P1 -∗ P2 -∗ typed_val_binop o t1 v1 t2 v2 t T)%I.
 
-  Class TypedBinOp (v1 : val) (P1 : assert) (v2 : val) (P2 : assert) (o : Cop.binary_operation) (ot1 ot2 : Ctypes.type) : Type :=
-    typed_bin_op_proof T : iProp_to_Prop (typed_bin_op v1 P1 v2 P2 o ot1 ot2 T).
+  Class TypedBinOp (v1 : val) (P1 : assert) (v2 : val) (P2 : assert) (o : Cop.binary_operation) (ot1 ot2 ot: Ctypes.type) : Type :=
+    typed_bin_op_proof T : iProp_to_Prop (typed_bin_op v1 P1 v2 P2 o ot1 ot2 ot T).
 
   Definition typed_val_unop op t v (T : val → type → assert) : assert :=
-    (∀ Φ, (∀ v (ty : type), ∃ cty, ⎡(valinject cty v) ◁ᵥ|cty| ty⎤ -∗ T v ty -∗ Φ v) -∗ wp_unop ⊤ op t v Φ).
+    (∀ Φ, (∀ v (ty : type), ∃ cty, ⎡v ◁ᵥₐₗ|cty| ty⎤ -∗ T v ty -∗ Φ v) -∗ wp_unop ⊤ op t v Φ).
   Global Arguments typed_val_unop _ _ _ _%_I.
 
   Definition typed_un_op (v : val) (P : assert) (o : Cop.unary_operation) (ot : Ctypes.type) (T : val → type → assert) : assert :=
@@ -280,7 +280,7 @@ Section judgements.
 
   (* FIXME this probably does not work; maybe providing a list of cty?  *)
   Definition typed_exprs f (el : list expr) (tl : list Ctypes.type) (T : list val → list type → assert) : assert :=
-    (∀ Φ, (∀ vl (tys : list type), ([∗ list] v;ty∈vl;tys, ∃ cty, ⎡(valinject cty v) ◁ᵥ|cty| ty⎤) -∗ T vl tys -∗ Φ vl) -∗ wp_exprs ge ⊤ f el tl Φ).
+    (∀ Φ, (∀ vl (tys : list type), ([∗ list] v;ty∈vl;tys, ∃ cty, ⎡v ◁ᵥₐₗ|cty| ty⎤) -∗ T vl tys -∗ Φ vl) -∗ wp_exprs ge ⊤ f el tl Φ).
   Global Arguments typed_exprs _ _ _ _%_I.
 
   (* can we rewrite this to take vals directly after all? We'd have to replace typed_stmt with sufficient
@@ -326,7 +326,7 @@ Section judgements.
   Definition typed_write f (atomic : bool) (e : expr) (ot : Ctypes.type) (v : val) (ty : type) (T : assert) : assert :=
     let E := if atomic then ∅ else ⊤ in
     (∀ (Φ: address->assert),
-        (∀ (l:address), (⎡(valinject ot v) ◁ᵥ|ot| ty⎤ ={⊤, E}=∗
+        (∀ (l:address), (⎡v ◁ᵥₐₗ|ot| ty⎤ ={⊤, E}=∗
                 <affine> ⌜(valinject ot v) `has_layout_val` ot⌝ ∗
                  ⎡ l ↦|ot| - ⎤ ∗
                 (* Ke : maybe we need later afterall because write is only done a write statement after? *)
@@ -384,7 +384,7 @@ Definition typed_read f (atomic : bool) (e : expr) (ot : Ctypes.type) (memcast :
   Definition typed_write_end (atomic : bool) (E : coPset) (ot : Ctypes.type) (v1 : val) (ty1 : type) (l2 : address) (β2 : own_state) (ty2 : type) (T : type → assert) : assert :=
     let E' := if atomic then ∅ else E in
     (⎡l2 ◁ₗ{β2} ty2⎤ -∗ 
-    (⎡(valinject ot v1) ◁ᵥ|ot| ty1⎤ ={E, E'}=∗
+    (⎡v1 ◁ᵥₐₗ|ot| ty1⎤ ={E, E'}=∗
        <affine> ⌜(valinject ot v1) `has_layout_val` ot⌝ ∗
       ⎡ l2↦|ot| - ⎤ ∗ 
       ▷ (⎡ l2 ↦|ot| (valinject ot v1) ⎤ ={E', E}=∗ ∃ ty3, ⎡l2 ◁ₗ{β2} ty3⎤ ∗ T ty3)))%I.
@@ -543,8 +543,8 @@ Global Hint Mode SimpleSubsumePlace + + + + + ! - : typeclass_instances.
 Global Hint Mode SimpleSubsumeVal + + + + + ! ! - : typeclass_instances.
 Global Hint Mode TypedIf + + + + + : typeclass_instances.
 (* Global Hint Mode TypedAssert + + + + + + : typeclass_instances. *)
-Global Hint Mode TypedValue + + + + + : typeclass_instances.
-Global Hint Mode TypedBinOp + + + + + + + + + + + + : typeclass_instances.
+Global Hint Mode TypedValue + + + + + + : typeclass_instances.
+Global Hint Mode TypedBinOp + + + + + + + + + + + + + : typeclass_instances.
 Global Hint Mode TypedUnOp + + + + + + + + : typeclass_instances.
 Global Hint Mode TypedCall + + + + + + + + + + : typeclass_instances.
 (*Global Hint Mode TypedCopyAllocId + + + + + + + : typeclass_instances. *)
@@ -601,11 +601,11 @@ Section proper.
   (** wand lemmas *)
   Lemma typed_val_expr_wand f e T1 T2:
     typed_val_expr ge f e T1 -∗
-    (∀ cty v ty, T1 cty v ty -∗ T2 cty v ty) -∗
+    (∀ v ty, T1 v ty -∗ T2 v ty) -∗
     typed_val_expr ge f e T2.
   Proof.
     iIntros "He HT" (Φ) "HΦ".
-    iApply "He". iIntros (cty v ty) "Hv Hty".
+    iApply "He". iIntros (v ty) "Hv Hty".
     iApply ("HΦ" with "Hv"). by iApply "HT".
   Qed.
 
@@ -621,11 +621,11 @@ Section proper.
       (iDestruct "HT" as "[_ HT]"; by iApply "HT") || (iDestruct "HT" as "[HT _]"; by iApply "HT")).
   Qed.
 
-  Lemma typed_bin_op_wand v1 P1 Q1 v2 P2 Q2 op ot1 ot2 T:
-    typed_bin_op ge v1 Q1 v2 Q2 op ot1 ot2 T -∗
+  Lemma typed_bin_op_wand v1 P1 Q1 v2 P2 Q2 op ot1 ot2 ot T:
+    typed_bin_op ge v1 Q1 v2 Q2 op ot1 ot2 ot T -∗
     (P1 -∗ Q1) -∗
     (P2 -∗ Q2) -∗
-    typed_bin_op ge v1 P1 v2 P2 op ot1 ot2 T.
+    typed_bin_op ge v1 P1 v2 P2 op ot1 ot2 ot T.
   Proof.
     iIntros "H Hw1 Hw2 H1 H2".
     iApply ("H" with "[Hw1 H1]"); [by iApply "Hw1"|by iApply "Hw2"].
@@ -640,12 +640,12 @@ Section proper.
   Qed.
 
   Lemma type_val_expr_mono_strong f e T :
-    typed_val_expr ge f e (λ cty v ty,
-      ∃ ty', subsume ⎡(valinject cty v) ◁ᵥ|cty| ty⎤ (λ _ : unit, ⎡(valinject cty v) ◁ᵥ|cty| ty'⎤) (λ _, T cty v ty'))%I
+    typed_val_expr ge f e (λ v ty,
+      ∃ ty', subsume ⎡v ◁ᵥₐₗ|typeof e| ty⎤ (λ _ : unit, ⎡v ◁ᵥₐₗ|typeof e| ty'⎤) (λ _, T v ty'))%I
     -∗ typed_val_expr ge f e T.
   Proof.
     iIntros "HT". iIntros (Φ) "HΦ".
-    iApply "HT". iIntros (cty v ty) "Hv HT".
+    iApply "HT". iIntros (v ty) "Hv HT".
     iDestruct "HT" as (ty') "HT".
     iPoseProof ("HT" with "Hv") as (?) "[Hv HT']".
     iApply ("HΦ" with "Hv HT'").
@@ -806,7 +806,7 @@ Global Typeclasses Opaque typed_write_end.*)
 Definition FindLoc `{!typeG OK_ty Σ} {cs : compspecs} (l : address) :=
   {| fic_A := own_state * type; fic_Prop '(β, ty):= (l ◁ₗ{β} ty)%I; |}.
 Definition FindVal `{!typeG OK_ty Σ} {cs : compspecs} cty (v : val) : @find_in_context_info assert :=
-  {| fic_A := type; fic_Prop ty := ⎡(valinject cty v) ◁ᵥ|cty| ty⎤%I; |}.
+  {| fic_A := type; fic_Prop ty := ⎡v ◁ᵥₐₗ|cty| ty⎤%I; |}.
 Definition FindValP {B : bi} (v : val) :=
   {| fic_A := B; fic_Prop P := P; |}.
 Definition FindValOrLoc {Σ} (v : val) (l : address) :=
@@ -820,8 +820,8 @@ Global Typeclasses Opaque FindLoc FindVal FindValP FindValOrLoc FindLocInBounds 
 (** setup instance generation *)
 Ltac generate_i2p_instance_to_tc_hook arg c ::=
   lazymatch c with
-  | typed_value ?x => constr:(TypedValue x)
-  | typed_bin_op ?x1 ?x2 ?x3 ?x4 ?x5 ?x6 ?x7 ?x8 => constr:(TypedBinOp x1 x2 x3 x4 x5 x6 x7 x8)
+  | typed_value ?cty ?x => constr:(TypedValue cty x)
+  | typed_bin_op ?x1 ?x2 ?x3 ?x4 ?x5 ?x6 ?x7 ?x8 ?x9 => constr:(TypedBinOp x1 x2 x3 x4 x5 x6 x7 x8 x9)
   | typed_un_op ?x1 ?x2 ?x3 ?x4 => constr:(TypedUnOp x1 x2 x3 x4)
 (*  | typed_call ?x1 ?x2 ?x3 ?x4 => constr:(TypedCall x1 x2 x3 x4)
   | typed_copy_alloc_id ?x1 ?x2 ?x3 ?x4 ?x5 => constr:(TypedCopyAllocId x1 x2 x3 x4 x5)
@@ -852,7 +852,7 @@ Section typing.
   Global Existing Instance find_in_context_type_loc_id_inst | 1.
 
   Lemma find_in_context_type_val_id cty v T:
-    (∃ ty, ⎡(valinject cty v) ◁ᵥ|cty| ty⎤ ∗ T ty)
+    (∃ ty, ⎡v ◁ᵥₐₗ|cty| ty⎤ ∗ T ty)
     ⊢ find_in_context (FindVal cty v) T.
   Proof. iDestruct 1 as (ty) "[Hl HT]". iExists _ => /=. iFrame. Qed.
   Definition find_in_context_type_val_id_inst :=
@@ -860,7 +860,7 @@ Section typing.
   Global Existing Instance find_in_context_type_val_id_inst | 1.
 
   Lemma find_in_context_type_val_P_id cty v T:
-    (∃ ty, (valinject cty v) ◁ᵥ|cty| ty ∗ T ((valinject cty v) ◁ᵥ|cty| ty))
+    (∃ ty, v ◁ᵥₐₗ|cty| ty ∗ T (v ◁ᵥₐₗ|cty| ty))
     ⊢ find_in_context (FindValP v) T.
   Proof. iDestruct 1 as (ty) "[Hl HT]". iExists (ty_own_val ty _ _) => /=. iFrame. Qed.
   Definition find_in_context_type_val_P_id_inst :=
@@ -876,7 +876,7 @@ Section typing.
   Global Existing Instance find_in_context_type_val_P_loc_id_inst | 10.
 
   Lemma find_in_context_type_val_or_loc_P_id_val cty (v : val) (l : address) T:
-    (∃ ty, (valinject cty v) ◁ᵥ|cty| ty ∗ T ((valinject cty v) ◁ᵥ|cty| ty))
+    (∃ ty, v ◁ᵥₐₗ|cty| ty ∗ T (v ◁ᵥₐₗ|cty| ty))
     ⊢ find_in_context (FindValOrLoc v l) T.
   Proof. iDestruct 1 as (ty) "[Hl HT]". iExists (ty_own_val ty _ _) => /=. iFrame. Qed.
   Definition find_in_context_type_val_or_loc_P_id_val_inst :=
@@ -1037,7 +1037,7 @@ Section typing.
   Global Existing Instance simplify_place_refine_l_inst.
 
   Lemma simplify_val_refine_l A (ty : rtype A) cty v T:
-    (∀ x, (valinject cty v) ◁ᵥ|cty| (x @ ty) -∗ T) ⊢ simplify_hyp ((valinject cty v) ◁ᵥ|cty| ty) T.
+    (∀ x, v ◁ᵥₐₗ|cty| (x @ ty) -∗ T) ⊢ simplify_hyp (v ◁ᵥₐₗ|cty| ty) T.
   Proof.
     iIntros "HT Hl". unfold ty_of_rty; simpl_type. iDestruct "Hl" as (x) "Hv". by iApply "HT".
   Qed.
@@ -1053,7 +1053,7 @@ Section typing.
   Global Existing Instance simplify_goal_place_refine_r_inst.
 
   Lemma simplify_goal_val_refine_r A (ty : rtype A) cty v T :
-    (∃ x, (valinject cty v) ◁ᵥ|cty| (x @ ty) ∗ T) ⊢ simplify_goal ((valinject cty v) ◁ᵥ|cty| ty) T.
+    (∃ x, v ◁ᵥₐₗ|cty| (x @ ty) ∗ T) ⊢ simplify_goal (v ◁ᵥₐₗ|cty| ty) T.
   Proof. iDestruct 1 as (x) "[? $]". by iExists _. Qed.
   Definition simplify_goal_val_refine_r_inst := [instance simplify_goal_val_refine_r with 10%N].
   Global Existing Instance simplify_goal_val_refine_r_inst.
@@ -1095,7 +1095,7 @@ Section typing.
   Global Existing Instance simple_subsume_place_to_subsume_inst.
 
   Lemma simple_subsume_val_to_subsume A cty v ty1 ty2 P `{!∀ x, SimpleSubsumeVal cty ty1 (ty2 x) (P x)} T:
-    (∃ x, P x ∗ T x) ⊢ subsume ((valinject cty v) ◁ᵥ|cty| ty1) (λ x : A, (valinject cty v) ◁ᵥ|cty| ty2 x) T.
+    (∃ x, P x ∗ T x) ⊢ subsume (v ◁ᵥₐₗ|cty| ty1) (λ x : A, v ◁ᵥₐₗ|cty| ty2 x) T.
   Proof. iIntros "[% [HP ?]] Hv". iExists _. iFrame. iApply (@simple_subsume_val with "HP Hv"). Qed.
   Definition simple_subsume_val_to_subsume_inst := [instance simple_subsume_val_to_subsume].
   Global Existing Instance simple_subsume_val_to_subsume_inst.
@@ -1123,9 +1123,9 @@ Section typing.
   (* This must be an Hint Extern because an instance would be a big slowdown. *)
   Definition subtype_var_inst := [instance @subtype_var].
 
-  Lemma typed_binop_simplify ge v1 P1 v2 P2 o1 o2 ot1 ot2 {SH1 : SimplifyHyp P1 o1} {SH2 : SimplifyHyp P2 o2} `{!TCOneIsSome o1 o2} op T:
-    let G1 := (SH1 (find_in_context (FindValP v1) (λ P, typed_bin_op ge v1 P v2 P2 op ot1 ot2 T))).(i2p_P) in
-    let G2 := (SH2 (find_in_context (FindValP v2) (λ P, typed_bin_op ge v1 P1 v2 P op ot1 ot2 T))).(i2p_P) in
+  Lemma typed_binop_simplify ge v1 P1 v2 P2 o1 o2 ot1 ot2 ot {SH1 : SimplifyHyp P1 o1} {SH2 : SimplifyHyp P2 o2} `{!TCOneIsSome o1 o2} op T:
+    let G1 := (SH1 (find_in_context (FindValP v1) (λ P, typed_bin_op ge v1 P v2 P2 op ot1 ot2 ot T))).(i2p_P) in
+    let G2 := (SH2 (find_in_context (FindValP v2) (λ P, typed_bin_op ge v1 P1 v2 P op ot1 ot2 ot T))).(i2p_P) in
     let G :=
        match o1, o2 with
      | Some n1, Some n2 => if (n2 ?= n1)%N is Lt then G2 else G1
@@ -1133,7 +1133,7 @@ Section typing.
      | _, _ => G2
        end in
     G
-    ⊢ typed_bin_op ge v1 P1 v2 P2 op ot1 ot2 T.
+    ⊢ typed_bin_op ge v1 P1 v2 P2 op ot1 ot2 ot T.
   Proof.
     iIntros "/= Hs Hv1 Hv2".
     destruct o1 as [n1|], o2 as [n2|] => //. 1: case_match.
@@ -1295,17 +1295,16 @@ Section typing.
   Lemma type_assign Espec ge f e1 e2 (T: option val -> type -> assert):
     type_is_by_value (typeof e1) = true ->
     type_is_volatile (typeof e1) = false ->
-    typed_val_expr ge f (Ecast e2 (typeof e1)) (λ cty v ty,
-      <affine> ⌜cty = typeof e1⌝ ∗
-      <affine> ⌜tc_val' cty v⌝ ∗
-       typed_write ge f false e1 cty v ty (T None tytrue))
+    typed_val_expr ge f (Ecast e2 (typeof e1)) (λ v ty,
+      <affine> ⌜tc_val' (typeof e1) v⌝ ∗
+       typed_write ge f false e1 (typeof e1) v ty (T None tytrue))
     ⊢ typed_stmt Espec ge (Sassign e1 e2) f T.
   Proof.
     intros.
     unfold typed_stmt.
     rewrite -wp_store.
     iIntros "H". iApply "H".
-    iIntros (cty v ty) "H (-> & % & ty_write)".
+    iIntros (v ty) "H (% & ty_write)".
     iSplit; [done|].
     iApply wp_lvalue_mono.
     { intros; apply derives_refl. }
@@ -1330,7 +1329,7 @@ Section typing.
   (* sets any v' to v *)
   Lemma type_set Espec ge f (id:ident) e v' (T: option val -> type -> assert):
     typed_val_expr ge f e (λ v ty, <affine> ⌜v ≠ Vundef⌝ ∗ env.temp id v' ∗ 
-                            (⎡v ◁ᵥ ty⎤ -∗ env.temp id v -∗ T None tytrue))%I
+                            (⎡v ◁ᵥₐₗ|typeof e| ty⎤ -∗ env.temp id v -∗ T None tytrue))%I
       ⊢ typed_stmt Espec ge (Sset id e) f T.
   Proof.
     iIntros "He".
@@ -1362,8 +1361,8 @@ Section typing.
     split; auto.
   Qed.
 
-  Lemma type_return_none Espec ge f (T : option val → type -> assert) ty:
-    ⎡Vundef ◁ᵥ ty⎤ ∗ T (Some Vundef) ty
+  Lemma type_return_none Espec ge f (T : option val → type -> assert) cty ty:
+    ⎡Vundef ◁ᵥₐₗ|cty| ty⎤ ∗ T (Some Vundef) ty
     ⊢ typed_stmt Espec ge (Sreturn $ None) f T.
   Proof.
     unfold typed_stmt.
@@ -1373,7 +1372,7 @@ Section typing.
   Qed.
 
   Lemma type_if Espec ge f e s1 s2 R:
-    typed_val_expr ge f e (λ v ty, typed_if (typeof e) v ⎡v ◁ᵥ ty⎤
+    typed_val_expr ge f e (λ v ty, typed_if (typeof e) v ⎡v ◁ᵥₐₗ|typeof e| ty⎤
           (⎡valid_val v⎤) (typed_stmt Espec ge s1 f R) (typed_stmt Espec ge s2 f R))
     ⊢ typed_stmt Espec ge (Sifthenelse e s1 s2) f R.
   Proof.
@@ -1496,9 +1495,9 @@ Qed.
   Qed.*)
 
   (*** expressions *)
-  Lemma type_val_context v T:
-    (find_in_context (FindVal v) T)
-    ⊢ typed_value v T.
+  Lemma type_val_context cty v T:
+    (find_in_context (FindVal cty v) T)
+    ⊢ typed_value cty v T.
   Proof.
     iDestruct 1 as (ty) "[Hv HT]". simpl in *.
     iExists _. iFrame.
@@ -1506,17 +1505,18 @@ Qed.
   Definition type_val_context_inst := [instance type_val_context].
   Global Existing Instance type_val_context_inst | 100.
 
-  Lemma type_const_int ge f i t T:
-    typed_value (Vint i) (T (Vint i))
+  Lemma type_const_int ge f i T t:
+    typed_value t (Vint i) (T (Vint i))
     ⊢ typed_val_expr ge f (Econst_int i t) T.
   Proof.
     iIntros "HP" (Φ) "HΦ".
     iDestruct "HP" as (ty) "[Hv HT]".
-    by iApply wp_const_int; iApply ("HΦ" with "[$]").
+    iApply wp_const_int. iApply ("HΦ" with "[Hv] HT").
+    rewrite /typeof //.
   Qed.
 
   Lemma type_const_long ge f i t T:
-    typed_value (Vlong i) (T (Vlong i))
+    typed_value t (Vlong i) (T (Vlong i))
     ⊢ typed_val_expr ge f (Econst_long i t) T.
   Proof.
     iIntros "HP" (Φ) "HΦ".
@@ -1525,7 +1525,7 @@ Qed.
   Qed.
 
   Lemma type_const_float ge f i t T:
-    typed_value (Vfloat i) (T (Vfloat i))
+    typed_value t (Vfloat i) (T (Vfloat i))
     ⊢ typed_val_expr ge f (Econst_float i t) T.
   Proof.
     iIntros "HP" (Φ) "HΦ".
@@ -1534,7 +1534,7 @@ Qed.
   Qed.
 
   Lemma type_const_single ge f i t T:
-    typed_value (Vsingle i) (T (Vsingle i))
+    typed_value t (Vsingle i) (T (Vsingle i))
     ⊢ typed_val_expr ge f (Econst_single i t) T.
   Proof.
     iIntros "HP" (Φ) "HΦ".
@@ -1542,8 +1542,12 @@ Qed.
     by iApply wp_const_single; iApply ("HΦ" with "[$]").
   Qed.
 
+
   Lemma type_bin_op ge f o e1 e2 ot T:
-    typed_val_expr ge f e1 (λ v1 ty1, typed_val_expr ge f e2 (λ v2 ty2, typed_bin_op ge v1 ⎡v1 ◁ᵥ ty1⎤ v2 ⎡v2 ◁ᵥ ty2⎤ o (typeof e1) (typeof e2) T))
+    typed_val_expr ge f e1 (λ v1 ty1,
+      typed_val_expr ge f e2 (λ v2 ty2,
+        typed_bin_op ge v1 ⎡v1 ◁ᵥₐₗ|typeof e1| ty1⎤ 
+                        v2 ⎡v2 ◁ᵥₐₗ|typeof e2| ty2⎤ o (typeof e1) (typeof e2) ot T))
     ⊢ typed_val_expr ge f (Ebinop o e1 e2 ot) T.
   Proof.
     iIntros "He1" (Φ) "HΦ".
@@ -1553,18 +1557,19 @@ Qed.
   Qed.
 
   Lemma type_un_op ge f o e ot T:
-    typed_val_expr ge f e (λ v ty, typed_un_op v ⎡v ◁ᵥ ty⎤ o (typeof e) T)
+    typed_val_expr ge f e (λ v ty, typed_un_op v ⎡v ◁ᵥₐₗ|typeof e| ty⎤ o (typeof e) T)
     ⊢ typed_val_expr ge f (Eunop o e ot) T.
   Proof.
     iIntros "He" (Φ) "HΦ".
     iApply wp_unop_rule. iApply "He". iIntros (v ty) "Hv Hop".
     rewrite /typed_un_op /typed_val_unop.
-    by iApply ("Hop" with "Hv").
+    iApply ("Hop" with "Hv").
+    rewrite /typeof //. iIntros; iExists _; iApply "HΦ".
   Qed.
 
-  Lemma type_tempvar ge f _x v c_ty T ty:
-     env.temp _x v ∗ (env.temp _x v -∗ ⎡ v ◁ᵥ ty ⎤ ∗ T v ty)
-    ⊢ typed_val_expr ge f (Etempvar _x c_ty) T.
+  Lemma type_tempvar ge f _x v cty T ty:
+     env.temp _x v ∗ (env.temp _x v -∗ ⎡v ◁ᵥₐₗ|cty| ty⎤ ∗ T v ty)
+    ⊢ typed_val_expr ge f (Etempvar _x cty) T.
   Proof.
     iIntros "(Hx & HT)" (Φ) "HΦ".
     iApply wp_tempvar_local.
@@ -1810,8 +1815,8 @@ Qed.
     `{!Copyable ty}
     `{!TCDone (ty2.(ty_has_op_type) ot MCNone)} :-
       exhale <affine> ⌜ty.(ty_has_op_type) ot MCNone⌝;
-      inhale ⎡v ◁ᵥ ty⎤;
-      ∀ v', inhale ⎡v' ◁ᵥ ty2⎤; (* FIXME this is probably not needed; can we not inhale this? *)
+      inhale ⎡v ◁ᵥₐₗ|ot| ty⎤;
+      inhale ∃ v', ⎡v' ◁ᵥ|ot| ty2⎤;
       return T ty.
   Proof.
     unfold typed_write_end, TCDone => ??. iDestruct 1 as (?) "HT".
@@ -1821,12 +1826,14 @@ Qed.
     iDestruct (ty_size_eq with "Hv'") as %?; [done|].
     iDestruct (ty_size_eq with "Hv") as %?; [done|].
     iApply fupd_mask_intro; [destruct a; solve_ndisj|]. iIntros "Hmask".
-    iSplit; [done|]. iSplitL "Hl". { iExists _. by iFrame. }
+    iSplit; [done|]. iSplitL "Hl". 
+    { rewrite mapsto_layout_iff_mapsto_and_layout. iExists _. iSplit;done. }
     iIntros "!# Hl". iMod "Hmask". iModIntro.
     iExists _.
-     iDestruct ("HT" with "Hv") as "HT".
-     iDestruct ("HT" $! v' with "Hv'") as "$".
-     by iApply (ty_ref with "[] Hl Hv").
+    iPoseProof (ty_ref with "[] Hl Hv") as "$"; try done.
+    rewrite /ty_own_val_at.
+    iDestruct ("HT" with "Hv [Hv']") as "HT"; try done.
+    iExists _; done.
   Qed.
   Definition type_write_own_copy_inst := [instance type_write_own_copy].
   Global Existing Instance type_write_own_copy_inst | 20.
